---
title: Proof using Set Theory
permalink: /docs/proof-set-theory/
---

## Seven-minute lecture

<iframe width="100%" height="400px" src="https://www.youtube-nocookie.com/embed/X_f8upZKcKc" frameborder="0" allow="accelerometer; autoplay; encrypted-media; gyroscope; picture-in-picture" allowfullscreen></iframe>

You can also view this video [on YouTube](https://youtu.be/X_f8upZKcKc)

## Questions

### 1. Check your understanding
Prove that Law 6.5 Holds. Where set R, S and T are defined by extension as:

    R = a, b, c
    S = a, b, c, d, e
    T = {c, d, e, f}

By applying it to calculate the following relations:

1. R\(S ∩ T) = (R\S) ∪ (R\T)
Hint: If you calculate the left side of the = and then the right side and the
results match then you’ve proven that the Law holds

Applying the Laws: We can apply the laws of set theory in the same
way we learned to apply the laws of propositional logic. For now lets do
this in plain English before we look at ways to do this through
equational reasoning.

1. Prove the following assertion with reference to the laws covered so far:

    S⊆∅⇒S=∅

## Summary

In this section we have learned about proof using set theory. Once you've finished the questions above, you're ready to move on to the [set theory challenges](./set-theory-challenges/).